Added evaluator logic
Added notation shortcuts
Made KripkeModels polymorphic types

Logic/DL/Semantics.lean
@@ -2,29 +2,48 @@ import Logic.DL.Syntax
 import Mathlib.Logic.Relation
 namespace Logic.DL
 
--- simple Kripke style structure, with natural numbers as states
-structure KripkeModel where
-  val : String → Nat → Prop --valuation function "does atomic prop hold in state?"
-  rel : Nat → Nat → Nat → Prop --transition function "atomic relation → state transition holds?"
+structure KripkeModel (RelType AtomType State: Type) where
+  val : AtomType → State → Prop --valuation function "does atomic prop hold in state?"
+  rel : RelType → State → State → Prop --transition function "atomic relation → state transition holds?"
 
 -- inductive relation evaluation over model
-def evalRel (M: KripkeModel) : Relation → Nat → Nat → Prop
+def evalRel (M: KripkeModel RelType AtomType State):
+  Relation RelType → State → State → Prop
   | Relation.relAtom a, s₀, s₁ => M.rel a s₀ s₁ --atomic defined by model.rel
-  | Relation.anywhere, _, _ => True --neglect reachability
-  | Relation.wild, s₀, s₁ => ∃ n, M.rel n s₀ s₁ --no notion of reachability in current implementation!
+  | Relation.emptyset, _, _ =>  False -- no transitions to another state at all
+  | Relation.wild, s₀, s₁ => ∃ a, M.rel a s₀ s₁
   | Relation.comp α β, s₀, s₁ => ∃ s₂, evalRel M α s₀ s₂ ∧ evalRel M β s₂ s₁
   | Relation.alt α β, s₀, s₁ => evalRel M α s₀ s₁ ∨ evalRel M β s₀ s₁
-  | Relation.iter α, s₀, s₁ => Relation.ReflTransGen (evalRel M α) s₀ s₁ --need transitive closure over α
+  | Relation.iter α, s₀, s₁ => Relation.ReflTransGen (evalRel M α) s₀ s₁
 
 --inductive formula evaluation over model
-def eval (M: KripkeModel) : DLForm → Nat → Prop
+def eval (M: KripkeModel RelType AtomType State) :
+  DLForm RelType AtomType → State → Prop
   | DLForm.atom a, s => M.val a s
   | DLForm.falsum, _ => False
   | DLForm.imp φ ψ, s => eval M φ s → eval M ψ s
   | DLForm.diamond α φ, s => ∃ s', evalRel M α s s' ∧ eval M φ s'
 
 
-def equiv (φ ψ: DLForm): Prop :=
-  ∀ (model: KripkeModel) (state: Nat), eval model φ state ↔ eval model ψ state
+def equiv {RelType AtomType State: Type} (φ ψ: DLForm RelType AtomType): Prop :=
+  ∀ (model: KripkeModel RelType AtomType State) (state: State), eval model φ state ↔ eval model ψ state
+
+def nonBranching (model: KripkeModel RelType AtomType State): Prop :=
+  ∀ (relAtom: RelType) (s₀ s₁ s₂: State), (model.rel relAtom s₀ s₁ ∧ model.rel relAtom s₀ s₂) → s₁ = s₂
+
+def validPDL {RelType AtomType State: Type} (φ: DLForm RelType AtomType): Prop :=
+  ∀ (model: KripkeModel RelType AtomType State) (s: State), eval model φ s
+
+def validDPDL {RelType AtomType State: Type} (φ: DLForm RelType AtomType): Prop :=
+  ∀ (model: KripkeModel RelType AtomType State) (s: State), nonBranching model → eval model φ s
+
+
+theorem validPDL_imp_validDPDL {RelType AtomType State: Type} (φ: DLForm RelType AtomType):
+  @validPDL RelType AtomType State φ → @validDPDL RelType AtomType State φ :=
+  by
+    intro validPDLH --assume pdl validity hypothesis
+    intro M s -- fix model, state
+    intro nBH -- assume nonBranching M
+    exact validPDLH M s -- apply hypothesis
 
 end Logic.DL
