Logic/DL/FinModelSemantics.lean
@@ -1,0 +1,128 @@
+import Logic.DL.Semantics
+import Mathlib.Data.Fintype.Basic
+import Mathlib.Data.Finset.Basic
+
+namespace Logic.DL
+
+
+--helpers to extract states and relations directly
+def relsFromList
+  {RelType State: Type}
+  [BEq RelType]
+  (rels : List (RelType × State × State)):
+  List RelType := (rels.map (λ (r, _, _) ↦ r)).eraseDups
+
+def statesFromList
+  {RelType State: Type}
+  [BEq State]
+  (rels: List (RelType × State × State)):
+  List State := (rels.map (λ (_, s₀, s₁) ↦ [s₀, s₁])).flatten.eraseDups
+
+--helpers to generate kripke model from lists
+def valFromList
+  {AtomType State: Type}
+  [DecidableEq AtomType][DecidableEq State]
+  (vals: List (AtomType × State)):
+  AtomType → State → Prop :=
+    λ atom state ↦ (atom, state) ∈ vals
+
+def relFromList
+  {RelType State: Type}
+  [DecidableEq RelType] [DecidableEq State]
+  (rels: List (RelType × State × State)):
+  RelType → State → State → Prop :=
+    λ relAtom s₁ s₂ ↦ (relAtom, s₁, s₂) ∈ rels
+
+def mkModel
+  {RelType AtomType State: Type}
+  [DecidableEq RelType] [DecidableEq AtomType] [DecidableEq State]
+  (valList: List (AtomType × State))
+  (relList: List (RelType × State × State)):
+  KripkeModel RelType AtomType State where
+    rel := relFromList relList
+    val := valFromList valList
+
+
+-- Decidable instances required for computation
+def valDecidable
+  {AtomType State: Type}
+  [DecidableEq AtomType] [DecidableEq State]
+  (xs: List (AtomType × State)):
+  ∀ atom state, Decidable ((valFromList xs) atom state) :=
+  by
+    intro atomType stateType
+    simp[valFromList]
+    infer_instance
+
+def relDecidable
+  {RelType State: Type}
+  [DecidableEq RelType] [DecidableEq State]
+  (xs: List (RelType × State × State)):
+  ∀ rel s s', Decidable ((relFromList xs) rel s s') :=
+  by
+    intro rel s s'
+    simp[relFromList]
+    infer_instance
+
+/-
+Boolean evaluation logic for finite models
+-/
+
+def evalRelB
+  {RelType AtomType State: Type}
+  [DecidableEq RelType] [DecidableEq State]
+  (M: KripkeModel RelType AtomType State)
+  (relDecidableH: ∀ rel s s', Decidable (M.rel rel s s'))
+  (states: List State) (rels: List RelType):
+  Relation RelType → State → State → Bool
+
+  | Relation.relAtom a, s₀, s₁ => @decide (M.rel a s₀ s₁) (relDecidableH a s₀ s₁)
+  | Relation.emptyset, _, _ => false
+  | Relation.wild, s₀, s₁ => rels.any (λ r ↦ @decide (M.rel r s₀ s₁) (relDecidableH r s₀ s₁))
+  | Relation.comp α β, s₀, s₁ => states.any (λ s₂ ↦
+                                                  evalRelB M relDecidableH states rels α s₀ s₂ &&
+                                                  evalRelB M relDecidableH states rels β s₂ s₁)
+  | Relation.alt α β, s₀, s₁ => evalRelB M relDecidableH states rels α s₀ s₁ ||
+                                evalRelB M relDecidableH states rels β s₀ s₁
+  | Relation.iter α, s₀, s₁ => decide (s₀ = s₁) --reflexive only → TODO: implement transitive!
+
+def evalB
+  {RelType AtomType State: Type}
+  [DecidableEq RelType] [DecidableEq State]
+  (M: KripkeModel RelType AtomType State)
+  (relDecidableH: ∀ rel s s', Decidable (M.rel rel s s'))
+  (valDecidableH: ∀ atom s, Decidable (M.val atom s))
+  (states: List State) (rels: List RelType):
+  DLForm RelType AtomType → State → Bool
+  
+  | DLForm.atom a, s => @decide (M.val a s) (valDecidableH a s)
+  | DLForm.falsum, _ => false
+  | DLForm.imp φ ψ, s => (! evalB M relDecidableH valDecidableH states rels φ s) ||
+                         (evalB M relDecidableH valDecidableH states rels ψ s)
+  | DLForm.diamond α φ, s => states.any (λ s' ↦
+                                              evalRelB M relDecidableH states rels α s s' &&
+                                              evalB M relDecidableH valDecidableH states rels φ s')
+
+
+--wrapper to evaluate directly over model defining rel/val in list notation
+def evalFromList
+  {RelType AtomType State: Type}
+  [DecidableEq RelType] [DecidableEq AtomType] [DecidableEq State]
+  [BEq RelType]
+  (vals: List (AtomType × State))
+  (rels: List (RelType × State × State))
+  (φ: DLForm RelType AtomType)
+  (s: State): Bool :=
+    let M := mkModel vals rels
+
+    --generate Decidable instances
+    let relH := relDecidable rels
+    let valH := valDecidable vals
+
+    --extract states/atomic relations in the model
+    let states := statesFromList rels
+    let atomicRels := relsFromList rels
+
+    evalB M relH valH states atomicRels φ s
+
+end Logic.DL
