Logic/DL/Notation.lean
@@ -1,0 +1,66 @@
+import Logic.DL.Syntax
+namespace Logic.DL
+
+/-
+# Remarks
+- This approach is only applicable when using the monomorphic DAForm, which fixes DynamicIndices and Atoms as DLForm Types
+- Any non atomic formula has to be parenthesized in order to ensure correct precedence - TODO!
+- Whitespaces need to be present between composition operator "." and the operands when using Nats, otherwise parsed as single number
+-/
+
+
+-- relevant coercions
+instance: Coe DynamicIndices (Relation DynamicIndices) where
+  coe α := Relation.relAtom α
+
+instance: OfNat DynamicIndices n where
+  ofNat := DynamicIndices.line n
+
+instance: OfNat (Relation DynamicIndices) n where
+  ofNat := Relation.relAtom (DynamicIndices.line n)
+
+instance: Coe String (DLForm DynamicIndices Atoms) where
+  coe p := DLForm.atom (Atoms.name p)
+
+instance: Coe String Atoms where
+  coe p := Atoms.name p
+
+--basic notations
+notation "$" => DynamicIndices.dollar
+notation "#" => DynamicIndices.hash
+
+notation "∅" => Relation.emptyset
+notation "•" => Relation.wild
+
+notation "⊥" => DLForm.falsum
+
+
+--relation operators
+notation:80 α " . " β  => Relation.comp (α: Relation DynamicIndices) (β: Relation DynamicIndices)
+notation:70 α " ∪ " β => Relation.alt (α: Relation DynamicIndices) (β: Relation DynamicIndices)
+notation:max α "*" => Relation.iter (α: Relation DynamicIndices)
+
+--formulas
+abbrev DAForm := DLForm DynamicIndices Atoms
+
+notation:60 φ " → " ψ => DLForm.imp (φ: DAForm) (ψ: DAForm)
+notation:90 "⟨" α "⟩" φ => DLForm.diamond (α: Relation DynamicIndices) (φ: DAForm)
+notation:90 "[" α "]" φ => box (α: Relation DynamicIndices) (φ: DAForm)
+notation:85 "¬" φ => not (φ: DAForm)
+notation:70 φ " ∧ " ψ => conj (φ: DAForm) (ψ: DAForm)
+notation:65 φ " ∨ " ψ => disj (φ: DAForm) (ψ: DAForm)
+
+
+#check [(0)*] "p"
+#check ¬⟨0 . $⟩ ¬"p" ∧ "q"
+#check ¬⟨0 . #⟩ (¬ "p") ∧ "q"
+#check "p" ∨ "q" ∧ "p"
+#check ("p" ∧ "q") ∨ "p"
+#check "p" ∧ ⊥ ∨ "p"
+#check "p" → "q"
+#check ⊥
+#check #
+#check ∅
+
+
+end Logic.DL
